AccessProp.v
@@ -6,7 +6,6 @@ From Elo Require Import Array.
 From Elo Require Import Core.
 From Elo Require Import Access.
 From Elo Require Import ValidAccesses.
-From Elo Require Import Compat.
 
 (* ------------------------------------------------------------------------- *)
 (* mem -- add                                                                *)
@@ -20,7 +19,8 @@ Proof.
   intros * Hnacc Hacc. remember (m +++ v) as m'.
   induction Hacc; inversion Heqm'; subst; inversion_not_access Hnacc.
   decompose sum (lt_eq_lt_dec ad' (length m)); subst; try lia;
-  do 2 simpl_array; eauto using access. simpl_array. inversion_access.
+  do 2 simpl_array; eauto using access. simpl_array. simpl in *.
+  inversion_access.
 Qed.
 
 (* ------------------------------------------------------------------------- *)
@@ -37,37 +37,37 @@ Proof.
   try (do 2 simpl_array); eauto using access.
 Qed.
 
-Local Lemma mem_set_acc' : forall m t ad ad' v,
+Local Lemma mem_set_acc' : forall m t ad ad' v V,
   ~ access m v ad ->
-  access m[ad' <- v] t ad ->
+  access m[ad' <- (v, V)] t ad ->
   access m t ad.
 Proof.
-  intros * Hnacc Hacc. remember (m[ad' <- v]) as m'.
+  intros * Hnacc Hacc. remember (m[ad' <- (v, V)]) as m'.
   induction Hacc; try rename IHHacc into IH;
   inversion_subst_clear Heqm'; eauto using access.
   match goal with |- access _ <{ & ?ad :: _ }> _ => rename ad into ad'' end.
   destruct (Nat.eq_dec ad' ad''); subst;
   try solve [do 2 simpl_array; eauto using access];
   destruct (Nat.eq_dec ad'' ad); subst; eauto using access.
-  auto_specialize. rewrite (get_set_eq TM_Unit) in IH. 1: contradiction.
+  auto_specialize. rewrite (get_set_eq memory_default) in IH. 1: contradiction.
   eapply not_le. intros Hlen. do 3 simpl_array. 
   eapply Nat.lt_eq_cases in Hlen as [? | ?]; subst;
-  do 2 simpl_array; inversion_access.
+  do 2 simpl_array; simpl in *; inversion_access.
 Qed.
 
 (* ------------------------------------------------------------------------- *)
 (* step-inherits-acc                                                         *)
 (* ------------------------------------------------------------------------- *)
 
-Lemma step_write_inherits_acc : forall m t t' ad ad' v,
-  access m[ad' <- v] t' ad ->
-  t --[EF_Write ad' v]--> t' ->
+Lemma step_write_inherits_acc : forall m t t' ad ad' v V,
+  access m[ad' <- (v, V)] t' ad ->
+  t --[EF_Write ad' v V]--> t' ->
   access m t ad.
 Proof.
   intros. induction_step; inversion_access; eauto using access;
   destruct (access_dec m v ad);
   eauto using mem_set_acc', access;
-  assert (forall t t', t --[EF_Write ad' v]--> t' -> access m t ad)
+  assert (forall t t', t --[EF_Write ad' v V]--> t' -> access m t ad)
     by (intros; induction_step; eauto using access);
   eauto using access.
 Qed.
@@ -106,7 +106,7 @@ Proof.
   inversion_not_access Hnacc; eauto using access.
   decompose sum (lt_eq_lt_dec ad' (length m)); subst;
   do 3 simpl_array; eauto using access; try contradiction.
-  auto_specialize. inversion_access.
+  auto_specialize. simpl in *. inversion_access.
 Qed.
 
 Lemma mem_add_nacc_length : forall m t v,
@@ -140,8 +140,7 @@ Proof.
   destruct (Nat.eq_dec ad ad'); subst; eauto using access.
   eapply access_mem; trivial.
   decompose sum (lt_eq_lt_dec ad' (length m)); subst;
-  simpl_array; trivial;
-  do 2 simpl_array; inversion_access.
+  simpl_array; trivial; do 2 simpl_array; simpl in *; inversion_access.
 Qed.
 
 (* ------------------------------------------------------------------------- *)
@@ -162,7 +161,7 @@ Proof.
 Qed.
 
 Lemma mem_set_preserves_acc2 : forall m t ad ad' v,
-  ~ access m m[ad'] ad ->
+  ~ access m m[ad'].tm ad ->
   access m t ad ->
   access m[ad' <- v] t ad.
 Proof.
@@ -186,21 +185,21 @@ Proof.
   do 2 simpl_array. eauto.
 Qed.
 
-Lemma mem_set_preserves_nacc : forall m t ad ad' v,
+Lemma mem_set_preserves_nacc : forall m t ad ad' v V,
   ~ access m v ad ->
   ~ access m t ad ->
-  ~ access m[ad' <- v] t ad.
+  ~ access m[ad' <- (v, V)] t ad.
 Proof.
   assert (ge_iff_le : forall m n, m >= n <-> n <= m)
     by (intros; split; destruct n; eauto).
   assert (forall m ad ad' v,
-    access m[ad' <- v] m[ad' <- v][ad'] ad ->
+    access m[ad' <- v] m[ad' <- v][ad'].tm ad ->
     ad' < length m). {
     intros * H. eapply not_ge. rewrite ge_iff_le. intros ?.
-    rewrite (get_set_invalid TM_Unit) in H; trivial. inversion H.
+    rewrite (get_set_invalid memory_default) in H; trivial. inversion H.
   }
 
-  intros * HnaccT HnaccV F. remember (m[ad' <- v]) as m'.
+  intros * HnaccT HnaccV F. remember (m[ad' <- (v, V)]) as m'.
   induction F; inversion_subst_clear Heqm'; eauto using access.
   match goal with _ : ~ access _ <{ & ?ad :: _ }> _ |- _ => 
     destruct (Nat.eq_dec ad' ad) as [? | Hneq]; subst;
@@ -213,17 +212,17 @@ Qed.
 (* Step                                                                      *)
 (* ------------------------------------------------------------------------- *)
 
-Lemma alloc_step_nacc_v : forall m t t' v,
+Lemma alloc_step_nacc_v : forall m t t' v V,
   valid_accesses m t ->
-  t --[EF_Alloc (length m) v]--> t' ->
+  t --[EF_Alloc (length m) v V]--> t' ->
   ~ access m v (length m).
 Proof.
   intros * Hva ?. induction_step; inversion_va; eauto using access.
   intros F. specialize (Hva (length m) F). lia.
 Qed.
 
-Lemma alloc_step_access_t'_ad : forall m t t' ad v,
-  t --[EF_Alloc ad v]--> t' ->
+Lemma alloc_step_access_t'_ad : forall m t t' ad v V,
+  t --[EF_Alloc ad v V]--> t' ->
   access m t' ad.
 Proof.
   intros. induction_step; eauto using access.
@@ -294,7 +293,7 @@ Qed.
 
 Lemma step_read_inherits_acc : forall m t t' ad ad',
   access m t' ad ->
-  t --[EF_Read ad' m[ad']]--> t' ->
+  t --[EF_Read ad' m[ad'].tm]--> t' ->
   access m t ad.
 Proof.
   intros * ? ?. induction_step;
@@ -304,7 +303,7 @@ Qed.
 
 Lemma step_read_preserves_not_access : forall m t t' ad ad',
   ~ access m t ad ->
-  t --[EF_Read ad' m[ad']]--> t' ->
+  t --[EF_Read ad' m[ad'].tm]--> t' ->
   ~ access m t' ad.
 Proof.
   intros * Hnacc ?. induction_step; inversion_not_access Hnacc;
@@ -365,10 +364,10 @@ Ltac solve_mstep_by H :=
 (* Alloc                                                                     *)
 (* ------------------------------------------------------------------------- *)
 
-Lemma step_alloc_preserves_acc : forall m t t' ad v,
+Lemma step_alloc_preserves_acc : forall m t t' ad v V,
   access m t ad ->
-  t --[EF_Alloc (length m) v]--> t' ->
-  access (m +++ v) t' ad.
+  t --[EF_Alloc (length m) v V]--> t' ->
+  access (m +++ (v, V)) t' ad.
 Proof.
   intros. induction_step; inversion_access;
   eauto using access, mem_add_preserves_access.
@@ -377,12 +376,12 @@ Proof.
   eauto using mem_add_preserves_access.
 Qed.
 
-Lemma step_alloc_preserves_nacc : forall m t t' ad v,
+Lemma step_alloc_preserves_nacc : forall m t t' ad v V,
   valid_accesses m t ->
   ad <> length m ->
   ~ access m t ad ->
-  t --[EF_Alloc (length m) v]--> t' ->
-  ~ access (m +++ v) t' ad.
+  t --[EF_Alloc (length m) v V]--> t' ->
+  ~ access (m +++ (v, V)) t' ad.
 Proof.
   intros * Hva ? Hnacc ?.
   induction_step; inversion_va; inversion_not_access Hnacc;
@@ -392,11 +391,11 @@ Proof.
   eauto using mem_add_nacc_lt, va_nacc_length.
 Qed.
 
-Lemma step_alloc_inherits_acc : forall m t t' ad v,
+Lemma step_alloc_inherits_acc : forall m t t' ad v V,
   valid_accesses m t ->
   ad <> length m ->
-  access (m +++ v) t' ad ->
-  t --[EF_Alloc (length m) v]--> t' ->
+  access (m +++ (v, V)) t' ad ->
+  t --[EF_Alloc (length m) v V]--> t' ->
   access m t ad.
 Proof.
   intros. induction_step;
@@ -405,11 +404,11 @@ Proof.
   eauto using mem_add_acc, va_nacc_length, access.
 Qed.
 
-Lemma step_alloc_creates_acc : forall ad v m t t',
+Lemma step_alloc_creates_acc : forall ad v m t t' V,
   valid_accesses m t ->
   ~ access m t ad ->
-  t --[EF_Alloc (length m) v]--> t' ->
-  access (m +++ v) t' ad ->
+  t --[EF_Alloc (length m) v V]--> t' ->
+  access (m +++ (v, V)) t' ad ->
   ad = length m.
 Proof.
   intros * ? Hnacc ? ?.
@@ -419,57 +418,25 @@ Proof.
   eauto using mem_add_nacc_lt, va_nacc_length.
 Qed.
 
-(* corollaries *)
-
-Corollary mstep_alloc_preserves_acc : forall m m' t t' ad ad' v,
-  access m t ad ->
-  m / t ==[EF_Alloc ad' v]==> m' / t' ->
-  access m' t' ad.
-Proof. solve_mstep_by step_alloc_preserves_acc. Qed.
-
-Corollary mstep_alloc_preserves_nacc : forall m m' t t' ad ad' v,
-  valid_accesses m t ->
-  ad <> length m ->
+Local Lemma step_write_value_nacc : forall m t t' ad ad' v V,
   ~ access m t ad ->
-  m / t ==[EF_Alloc ad' v]==> m' / t' ->
-  ~ access m' t' ad.
-Proof. solve_mstep_by step_alloc_preserves_nacc. Qed.
-
-Corollary mstep_alloc_inherits_acc : forall m m' t t' ad ad' v,
-  valid_accesses m t ->
-  ad <> ad' ->
-  access m' t' ad ->
-  m / t ==[EF_Alloc ad' v]==> m' / t' ->
-  access m t ad.
-Proof. solve_mstep_by step_alloc_inherits_acc. Qed.
-
-Corollary mstep_alloc_creates_acc : forall m m' t t' ad ad' v,
-  valid_accesses m t ->
-  ~ access m t ad ->
-  m / t ==[EF_Alloc ad' v]==> m' / t' ->
-  access (m +++ v) t' ad ->
-  ad = length m.
-Proof. solve_mstep_by step_alloc_creates_acc. Qed.
-
-Local Lemma step_write_value_nacc : forall m t t' ad ad' v,
-  ~ access m t ad ->
-  t --[EF_Write ad' v]--> t' ->
+  t --[EF_Write ad' v V]--> t' ->
   ~ access m v ad.
 Proof.
   intros. induction_step; eauto using access.
 Qed.
 
-Lemma step_write_requires_acc : forall m t t' ad v,
-  t --[EF_Write ad v]--> t' ->
+Lemma step_write_requires_acc : forall m t t' ad v V,
+  t --[EF_Write ad v V]--> t' ->
   access m t ad.
 Proof.
   intros. induction_step; eauto using access.
 Qed.
 
-Lemma step_write_preserves_nacc : forall m t t' ad ad' v,
+Lemma step_write_preserves_nacc : forall m t t' ad ad' v V,
   ~ access m t ad ->
-  t --[EF_Write ad' v]--> t' ->
-  ~ access m[ad' <- v] t' ad.
+  t --[EF_Write ad' v V]--> t' ->
+  ~ access m[ad' <- (v, V)] t' ad.
 Proof.
   intros * Hnacc ?. induction_step; 
   inversion_not_access Hnacc; eapply not_access_iff; eauto using not_access;
